CoherenceAlgo.v
@@ -1,46 +1,55 @@
 Require Import CSet Le.
 
 Require Import Plus Util AllInRel Map.
-Require Import Val Var Env EnvTy IL Liveness Coherence ParamsMatch Sim MoreList.
+Require Import Val Var Env EnvTy IL Liveness Coherence ParamsMatch Sim MoreList Restrict ILIToILF.
 
 Set Implicit Arguments.
 
-Definition addParam x (DL:list (live * params)) (AP:list (set var)) := 
-  zip (fun DL AP => if [x ∈ fst DL] then {{x}} ∪ AP else AP) DL AP.
+Definition addParam x (DL:list (live)) ZL (AP:list (set var)) := 
+  zip (fun (DLZ:live*params) AP => if [x ∈ fst DLZ \ of_list (snd DLZ)] 
+                   then {{x}} ∪ AP else AP) (zip pair DL ZL) AP.
 
-Definition addParams Z DL (AP:list (set var)) := 
-  fold_left (fun AP x => addParam x DL AP) Z AP.
-
+Definition addParams Z DL ZL (AP:list (set var)) := 
+  fold_left (fun AP x => addParam x DL ZL AP) Z AP.
 
 Definition killExcept f (AP:list (set var)) :=
-  mapi (fun n x => if [n = counted f] then x else ∅) AP.
+  mapi (fun n x => if [n = counted f] then Some x else None) AP.
 
+Definition ounion (s t: option (set var)) :=
+  match s, t with 
+    | Some s, Some t => Some (s ∪ t)
+    | Some s, None => Some s
+    | None, Some t => Some t
+    | _, _ => None
+  end.
 
-Fixpoint computeParameters (DL: list (set var * params)) (AP:list (set var)) 
+Fixpoint computeParameters (DL: list (set var)) (ZL:list params) (AP:list (set var)) 
          (s:stmt) (an:ann (set var)) {struct s}
-: ann (list var) * list (set var) :=
+: ann (list var) * list (option (set var)) :=
   match s, an with
     | stmtExp x e s, annExp _ an => 
-      let (ar, r) := computeParameters DL (addParam x DL AP) s an in
+      let (ar, r) := computeParameters DL ZL (addParam x DL ZL AP) s an in
       (annExp nil ar, r) 
     | stmtIf x s t, annIf _ ans ant => 
-      let (ars, rs) := computeParameters DL AP s ans in
-      let (art, rt) := computeParameters DL AP t ant in
-      (annIf nil ars art, zip union rs rt)
+      let (ars, rs) := computeParameters DL ZL AP s ans in
+      let (art, rt) := computeParameters DL ZL AP t ant in
+      (annIf nil ars art, zip ounion rs rt)
     | stmtGoto f Y, annGoto lv => (annGoto nil, killExcept f AP)
-    | stmtReturn x, annReturn _ => (annReturn nil, (mapi (fun _ _ => ∅) AP))
+    | stmtReturn x, annReturn _ => (annReturn nil, (mapi (fun _ _ => None) AP))
     | stmtLet Z s t, annLet lv ans ant =>
-      let DL' := (getAnn ans \ of_list Z, Z) in
+      let DL' := getAnn ans in
       let (ars, rs) := computeParameters (DL' :: DL) 
-                                        (∅ :: addParams Z DL AP)
+                                        (Z :: ZL)
+                                        (∅ :: addParams Z DL ZL AP)
                                         s
                                         ans in
       let (art, rt) := computeParameters (DL':: DL) 
+                                        (Z :: ZL)
                                         (∅:: AP) 
                                         t 
                                         ant in
-      let ur := zip union rs rt in
-      (annLet (to_list (hd (∅:set var) ur)) ars art, tl ur)
+      let ur := zip ounion rs rt in
+      (annLet (match (hd None ur) with Some s => to_list s | None => nil end) ars art, tl ur)
     | s, a => (annReturn nil, nil)
   end.
 
