IL/SimApx.v
@@ -1,0 +1,164 @@
+Require Import List Infra.Relations.
+Require Export Util Var Val Exp Env Map CSet AutoIndTac IL Sim.
+
+Set Implicit Arguments.
+Unset Printing Records.
+
+CoInductive simapx {S} `{StateType S} {S'} `{StateType S'}  : S -> S' -> Prop :=
+  | simS (σ1 σ1':S) (σ2 σ2':S') : (* result σ1 = result σ2 -> *) plus step σ1 σ1' -> plus step σ2 σ2' -> simapx σ1' σ2' -> simapx σ1 σ2
+  | simE (σ1 σ1':S) (σ2 σ2':S') 
+    : result σ1' = result σ2'
+      -> star step σ1 σ1'
+      -> star step σ2 σ2'
+      -> normal step σ1'
+      -> normal step σ2' -> simapx σ1 σ2
+  | simErr (σ1 σ1':S) (σ2:S') 
+    : result σ1' = None
+      -> star step σ1 σ1'
+      -> normal step σ1' -> simapx σ1 σ2.
+
+(** Simulation is an equivalence relation *)
+Lemma simapx_refl {S} `{StateType S} (σ:S)
+      : simapx σ σ.
+Proof.
+  revert σ. cofix.  
+  intros. destruct (step_dec σ). inv H0.
+  eapply simS; eauto using plusO.
+  eapply simE; eauto using star_refl.
+Qed.
+
+(** Transitivity is not obvious *)
+
+Definition apxbehave {S} `{StateType S} {S'} `{StateType S'} (σ1:S) (σ2:S') :=
+  (diverges step σ1 -> diverges step σ2) 
+  /\ (forall v, terminatesWith σ1 (Some v) -> terminatesWith σ2 (Some v)).
+
+Lemma apxbehave_reduction_closed {S} `{StateType S} {S'} `{StateType S'} 
+      (σ1 σ1':S) (σ2 σ2':S')
+  : apxbehave σ1 σ2
+    -> star step σ1 σ1' 
+    -> star step σ2 σ2'
+    -> apxbehave σ1' σ2'.
+Proof.
+  intros.
+  destruct H1. split; intros.
+  eapply diverges_star; eauto. eapply H1. eapply star_diverges; eauto.
+  eapply terminatesWith_star_2; eauto. eapply H4. eapply terminatesWith_star; eauto.
+Qed.
+
+Lemma simapx_codiverge' {S} `{StateType S} {S'} `{StateType S'} (σ1:S) (σ2:S')
+: simapx σ1 σ2 -> diverges step σ1 -> diverges (plus step) σ2.
+Proof.
+  revert σ1 σ2. cofix; intros.
+  intros.
+  inv H1. eapply DivergesI; eauto. eapply simapx_codiverge'; eauto.
+  eapply div_ext_plus; eauto. eapply step_functional.
+  exfalso. eapply normal_terminates in H6. 
+  eapply div_ext_star_2 in H2; eauto.
+  eapply divergence_or_termination; eassumption. eapply step_functional.
+  exfalso. eapply normal_terminates in H5. 
+  eapply div_ext_star_2 in H2; eauto.
+  eapply divergence_or_termination; eassumption. eapply step_functional.
+Qed.
+
+Lemma simapx_codiverge {S} `{StateType S} {S'} `{StateType S'} (σ1:S) (σ2:S')
+: simapx σ1 σ2 -> diverges step σ1 -> diverges step σ2.
+Proof.
+  intros. eapply div_plus. eapply (simapx_codiverge' H1 H2).
+Qed.
+
+Lemma codiverge_simapx {S} `{StateType S} {S'} `{StateType S'} (σ1:S) (σ2:S')
+: diverges step σ1 -> diverges step σ2 -> simapx σ1 σ2.
+Proof.
+  revert σ1 σ2. cofix; intros.
+  inv H1; inv H2.
+  eapply simS; eauto using plus.
+Qed.
+
+Lemma simapx_step_closed {S} `{StateType S} {S'} `{StateType S'} (σ1 σ1':S) (σ2:S')
+ : simapx σ1 σ2 -> step σ1 σ1' -> simapx σ1' σ2.
+Proof.
+  revert σ1 σ1' σ2. cofix; intros.
+  inv H1. destruct H3. inv H5. 
+  eapply simS. rewrite step_functional; eauto.
+  eapply plus_trans; eauto. eassumption.
+  eapply simE. eauto. rewrite step_functional; eauto. 
+  eapply star_trans; eauto using plus_star.
+  eauto. eauto. 
+  eapply simErr; eauto. rewrite step_functional; eauto.
+  eapply simS. rewrite step_functional; eauto. eassumption. eauto. 
+  eapply simE. eauto. destruct H4. exfalso; firstorder.
+  rewrite step_functional; eauto. eauto. eauto. eauto.
+  eapply simErr; eauto. destruct H4. exfalso; firstorder.
+  rewrite step_functional; eauto.
+Qed.
+
+Lemma simapx_coterminatesWith {S} `{StateType S} {S'} `{StateType S'} (σ1:S) (σ2:S')
+: simapx σ1 σ2 -> forall v, terminatesWith σ1 (Some v) -> terminatesWith σ2 (Some v).
+Proof.
+  intros. general induction H2. rewrite Heqo.
+  + inv H3. exfalso. eapply H1. destruct H0; firstorder. 
+    destruct H4. eapply terminatesWith_star; eauto. econstructor; eauto.
+    congruence. admit. admit.
+  + eapply IHterminatesWith. 
+    pose proof (simapx_step_closed _ H3 H0). eauto. reflexivity.
+Qed.
+
+Lemma coterminatesWith_simapx {S} `{StateType S} {S'} `{StateType S'} (σ1:S) (σ2:S') v
+: terminatesWith σ1 v -> terminatesWith σ2 v -> simapx σ1 σ2.
+Proof. 
+  intros. 
+  eapply terminatesWith_star_normal in H1.
+  eapply terminatesWith_star_normal in H2.
+  destruct H1, H2; dcr.
+  eapply simE; eauto using star. rewrite H6, H8; reflexivity.
+Qed.
+(*
+Lemma sim_apxbehave {S} `{StateType S} {S'} `{StateType S'} (σ1:S) (σ2:S')
+: simapx σ1 σ2 <-> apxbehave σ1 σ2.
+Proof.
+  split. unfold cobehave; split; intros.
+  + pose proof (simapx_codiverge H1 H2); eauto.
+  + eapply (simapx_coterminatesWith H1); eassumption.
+  + revert_all. cofix; intros. 
+    destruct (step_dec σ1) as [[]|]; destruct (step_dec σ2) as [[]|].
+    - eapply simS; try eapply plusO; try eassumption. 
+      eapply sim_apxbehave. eapply apxbehave_reduction_closed; eauto using star.
+    - pose proof (normal_terminates H3).
+      eapply terminatesWith_terminates in H4; destruct H4. 
+      destruct x0.
+      assert (terminatesWith σ1 (Some v)). eapply H1; eauto.
+      eapply coterminatesWith_sim; eauto.
+    - pose proof (normal_terminates H2). eapply terminatesWith_terminates in H4; destruct H4.
+      assert (terminatesWith σ2 x0). eapply H1; eauto.
+      eapply coterminatesWith_sim; eauto.
+    - pose proof (normal_terminates H2). eapply terminatesWith_terminates in H4; destruct H4.
+      assert (terminatesWith σ2 x). eapply H1; eauto.
+      eapply coterminatesWith_sim; eauto.
+Qed.
+
+Lemma cobehave_trans {S} `{StateType S} {S'} `{StateType S'} {S''} `{StateType S''} 
+(σ1:S) (σ2:S') (σ3:S'')
+: cobehave σ1 σ2 -> cobehave σ2 σ3 -> cobehave σ1 σ3.
+Proof. 
+  unfold cobehave; intros. destruct H2, H3; firstorder.
+Qed.
+
+Lemma sim_trans {S1} `{StateType S1} {S2} `{StateType S2} {S3} `{StateType S3}
+      (σ1:S1) (σ2:S2) (σ3:S3)
+  : sim σ1 σ2 -> sim σ2 σ3 -> sim σ1 σ3.
+Proof.
+  intros. 
+  rewrite sim_cobehave in H2. 
+  rewrite sim_cobehave in H3. 
+  rewrite sim_cobehave. 
+  pose proof (cobehave_trans H2 H3); eauto.
+Qed.
+*)
+
+(* 
+*** Local Variables: ***
+*** coq-load-path: (("../" "Lyn")) ***
+*** End: ***
+*)
+
